no longer axiomatize PatSyn

examples/ghc/manual/PatSyn.v
@@ -13,11 +13,18 @@ Require Coq.Program.Wf.
 (* Converted imports: *)
 
 Require BasicTypes.
+Require Data.Foldable.
+Require Data.Function.
+Require Data.Tuple.
 Require FieldLabel.
 Require GHC.Base.
+Require GHC.List.
 Require Name.
+Require OccName.
+Require Panic.
 Require Unique.
 Require Var.
+Import GHC.Base.Notations.
 
 (* Converted type declarations: *)
 
@@ -87,22 +94,25 @@ Definition psUnivTyVars (arg_0__ : PatSyn) :=
   psUnivTyVars.
 (* Midamble *)
 
-Instance Unique_PatSyn : Unique.Uniquable PatSyn := {}.
-Admitted.
 
 (* Converted value declarations: *)
 
-Instance Eq___PatSyn : GHC.Base.Eq_ PatSyn := {}.
-Proof.
-Admitted.
+Local Definition Uniquable__PatSyn_getUnique : PatSyn -> Unique.Unique :=
+  psUnique.
 
-Instance Uniquable__PatSyn : Unique.Uniquable PatSyn := {}.
-Proof.
-Admitted.
+Program Instance Uniquable__PatSyn : Unique.Uniquable PatSyn :=
+  fun _ k => k {| Unique.getUnique__ := Uniquable__PatSyn_getUnique |}.
 
-Instance NamedThing__PatSyn : Name.NamedThing PatSyn := {}.
-Proof.
-Admitted.
+Local Definition Eq___PatSyn_op_zeze__ : PatSyn -> PatSyn -> bool :=
+  Data.Function.on _GHC.Base.==_ Unique.getUnique.
+
+Local Definition Eq___PatSyn_op_zsze__ : PatSyn -> PatSyn -> bool :=
+  Data.Function.on _GHC.Base./=_ Unique.getUnique.
+
+Program Instance Eq___PatSyn : GHC.Base.Eq_ PatSyn :=
+  fun _ k =>
+    k {| GHC.Base.op_zeze____ := Eq___PatSyn_op_zeze__ ;
+         GHC.Base.op_zsze____ := Eq___PatSyn_op_zsze__ |}.
 
 (* Skipping instance Outputable__PatSyn of class Outputable *)
 
@@ -110,50 +120,119 @@ Admitted.
 
 (* Skipping instance Data__PatSyn of class Data *)
 
-Axiom mkPatSyn : Name.Name ->
-                 bool ->
-                 (list Var.TyVarBinder * unit)%type ->
-                 (list Var.TyVarBinder * unit)%type ->
-                 list unit ->
-                 unit ->
-                 (Var.Id * bool)%type ->
-                 option (Var.Id * bool)%type -> list FieldLabel.FieldLabel -> PatSyn.
+Definition mkPatSyn
+   : Name.Name ->
+     bool ->
+     (list Var.TyVarBinder * unit)%type ->
+     (list Var.TyVarBinder * unit)%type ->
+     list unit ->
+     unit ->
+     (Var.Id * bool)%type ->
+     option (Var.Id * bool)%type -> list FieldLabel.FieldLabel -> PatSyn :=
+  fun arg_0__ arg_1__ arg_2__ arg_3__ arg_4__ arg_5__ arg_6__ arg_7__ arg_8__ =>
+    match arg_0__
+        , arg_1__
+        , arg_2__
+        , arg_3__
+        , arg_4__
+        , arg_5__
+        , arg_6__
+        , arg_7__
+        , arg_8__ with
+    | name
+    , declared_infix
+    , pair univ_tvs req_theta
+    , pair ex_tvs prov_theta
+    , orig_args
+    , orig_res_ty
+    , matcher
+    , builder
+    , field_labels =>
+        MkPatSyn name (Unique.getUnique name) orig_args (Data.Foldable.length orig_args)
+                 declared_infix field_labels univ_tvs req_theta ex_tvs prov_theta orig_res_ty
+                 matcher builder
+    end.
 
-Axiom patSynName : PatSyn -> Name.Name.
+Definition patSynArgs : PatSyn -> list unit :=
+  psArgs.
 
-Axiom patSynIsInfix : PatSyn -> bool.
+Definition patSynArity : PatSyn -> BasicTypes.Arity :=
+  psArity.
 
-Axiom patSynArity : PatSyn -> BasicTypes.Arity.
+Definition patSynBuilder : PatSyn -> option (Var.Id * bool)%type :=
+  psBuilder.
 
-Axiom patSynArgs : PatSyn -> list unit.
+Definition patSynExTyVarBinders : PatSyn -> list Var.TyVarBinder :=
+  psExTyVars.
 
-Axiom patSynFieldLabels : PatSyn -> list FieldLabel.FieldLabel.
+Definition patSynExTyVars : PatSyn -> list Var.TyVar :=
+  fun ps => Var.binderVars (psExTyVars ps).
 
-Axiom patSynFieldType : PatSyn -> FieldLabel.FieldLabelString -> unit.
+Definition patSynFieldLabels : PatSyn -> list FieldLabel.FieldLabel :=
+  psFieldLabels.
 
-Axiom patSynUnivTyVarBinders : PatSyn -> list Var.TyVarBinder.
+Definition patSynFieldType : PatSyn -> FieldLabel.FieldLabelString -> unit :=
+  fun ps label =>
+    match Data.Foldable.find ((fun arg_0__ => arg_0__ GHC.Base.== label) GHC.Base.∘
+                              (FieldLabel.flLabel GHC.Base.∘ Data.Tuple.fst)) (GHC.List.zip (psFieldLabels ps)
+                                                                                            (psArgs ps)) with
+    | Some (pair _ ty) => ty
+    | None =>
+        Panic.panicStr (GHC.Base.hs_string__ "dataConFieldType") (GHC.Base.mappend
+                                                                  (Panic.noString ps) (Panic.noString label))
+    end.
 
-Axiom patSynExTyVars : PatSyn -> list Var.TyVar.
+Definition patSynIsInfix : PatSyn -> bool :=
+  psInfix.
 
-Axiom patSynExTyVarBinders : PatSyn -> list Var.TyVarBinder.
+Definition patSynMatcher : PatSyn -> (Var.Id * bool)%type :=
+  psMatcher.
 
-Axiom patSynSig : PatSyn ->
-                  (list Var.TyVar * unit * list Var.TyVar * unit * list unit * unit)%type.
+Definition patSynName : PatSyn -> Name.Name :=
+  psName.
 
-Axiom patSynMatcher : PatSyn -> (Var.Id * bool)%type.
+Local Definition NamedThing__PatSyn_getName : PatSyn -> Name.Name :=
+  patSynName.
 
-Axiom patSynBuilder : PatSyn -> option (Var.Id * bool)%type.
+Local Definition NamedThing__PatSyn_getOccName : PatSyn -> OccName.OccName :=
+  fun n => Name.nameOccName (NamedThing__PatSyn_getName n).
 
-Axiom tidyPatSynIds : (Var.Id -> Var.Id) -> PatSyn -> PatSyn.
+Program Instance NamedThing__PatSyn : Name.NamedThing PatSyn :=
+  fun _ k =>
+    k {| Name.getName__ := NamedThing__PatSyn_getName ;
+         Name.getOccName__ := NamedThing__PatSyn_getOccName |}.
 
-Axiom patSynInstArgTys : PatSyn -> list unit -> list unit.
+Definition patSynSig
+   : PatSyn ->
+     (list Var.TyVar * unit * list Var.TyVar * unit * list unit * unit)%type :=
+  fun '(MkPatSyn _ _ arg_tys _ _ _ univ_tvs req ex_tvs prov res_ty _ _) =>
+    pair (pair (pair (pair (pair (Var.binderVars univ_tvs) req) (Var.binderVars
+                            ex_tvs)) prov) arg_tys) res_ty.
 
-Axiom patSynInstResTy : PatSyn -> list unit -> unit.
+Definition patSynUnivTyVarBinders : PatSyn -> list Var.TyVarBinder :=
+  psUnivTyVars.
 
-(* pprPatSynType skipped *)
+Definition tidyPatSynIds : (Var.Id -> Var.Id) -> PatSyn -> PatSyn :=
+  fun arg_0__ arg_1__ =>
+    match arg_0__, arg_1__ with
+    | tidy_fn, (MkPatSyn _ _ _ _ _ _ _ _ _ _ _ matcher builder as ps) =>
+        let tidy_pr := fun '(pair id dummy) => pair (tidy_fn id) dummy in
+        let 'MkPatSyn psName_5__ psUnique_6__ psArgs_7__ psArity_8__ psInfix_9__
+           psFieldLabels_10__ psUnivTyVars_11__ psReqTheta_12__ psExTyVars_13__
+           psProvTheta_14__ psResultTy_15__ psMatcher_16__ psBuilder_17__ := ps in
+        MkPatSyn psName_5__ psUnique_6__ psArgs_7__ psArity_8__ psInfix_9__
+                 psFieldLabels_10__ psUnivTyVars_11__ psReqTheta_12__ psExTyVars_13__
+                 psProvTheta_14__ psResultTy_15__ (tidy_pr matcher) (GHC.Base.fmap tidy_pr
+                  builder)
+    end.
 
 (* External variables:
-     bool list op_zt__ option unit BasicTypes.Arity FieldLabel.FieldLabel
-     FieldLabel.FieldLabelString GHC.Base.Eq_ Name.Name Name.NamedThing
-     Unique.Uniquable Unique.Unique Var.Id Var.TyVar Var.TyVarBinder
+     None Some bool list op_zt__ option pair unit BasicTypes.Arity Data.Foldable.find
+     Data.Foldable.length Data.Function.on Data.Tuple.fst FieldLabel.FieldLabel
+     FieldLabel.FieldLabelString FieldLabel.flLabel GHC.Base.Eq_ GHC.Base.fmap
+     GHC.Base.mappend GHC.Base.op_z2218U__ GHC.Base.op_zeze__ GHC.Base.op_zeze____
+     GHC.Base.op_zsze__ GHC.Base.op_zsze____ GHC.List.zip Name.Name Name.NamedThing
+     Name.getName__ Name.getOccName__ Name.nameOccName OccName.OccName Panic.noString
+     Panic.panicStr Unique.Uniquable Unique.Unique Unique.getUnique
+     Unique.getUnique__ Var.Id Var.TyVar Var.TyVarBinder Var.binderVars
 *)
