examples/ghc/module-edits/PatSyn/midamble.v
@@ -1,2 +1,0 @@
-Instance Unique_PatSyn : Unique.Uniquable PatSyn := {}.
-Admitted.
